

Q1. Prove the following identities :

$$(i) (1 - \sin^2 \theta) \sec^2 \theta = 1 \quad (ii) \cos^2 \theta (1 + \tan^2 \theta) = 1 \quad (iii) \cos^2 \theta + \frac{1}{1 + \cot^2 \theta} = 1 \quad (iv) \frac{1}{\sec^2 \theta} + \frac{1}{\operatorname{cosec}^2 \theta} = 1$$

$$(v) \frac{\operatorname{cosec}^2 A}{1 + \cot^2 A} = 1 \quad (vi) \sin^2 \theta + \frac{1}{1 + \tan^2 \theta} = 1 \quad (vii) \sqrt{\frac{\tan^2 \theta}{1 + \tan^2 \theta}} = \sin \theta \quad (viii) \sqrt{\frac{\cot^2 \theta}{1 + \cot^2 \theta}} = \cos \theta$$

Q2. Simplify :

$$(i) \sin^2 \theta + \cos^2 \theta + \cot^2 \theta \quad (ii) \sin^2 A + \cos^2 A + \tan^2 A \quad (iii) \frac{1 + \tan^2 A}{1 + \cot^2 A} \quad (iv) 9(\sec^2 A - \tan^2 A)$$

$$(v) \cot^2 \theta - \frac{1}{\sin^2 \theta} \quad (vi) \tan^2 \theta - \frac{1}{\cos^2 \theta} \quad (vii) (1 + \tan^2 \theta)(1 + \sin \theta)(1 - \sin \theta)$$

$$(viii) (1 + \cot^2 \theta)(1 + \cos \theta)(1 - \cos \theta)$$



Ans 2. (i) $\operatorname{cosec}^2 \theta$ (ii) $\sec^2 A$ (iii) $\tan^2 A$ (iv) 9 (v) -1 (vi) -1 (vii) 1 (viii) 1

Q3. Prove the following identities :

$$(i) \frac{1}{1 + \sin \theta} + \frac{1}{1 - \sin \theta} = 2 \sec^2 \theta \quad (ii) \operatorname{cosec}^2 \theta + \sec^2 \theta = \operatorname{cosec}^2 \theta \cdot \sec^2 \theta$$

$$(iii) (\sec A + \tan A)(1 - \sin A) = \cos A \quad (iv) (1 + \tan \theta + \sec \theta)(1 + \cot \theta - \operatorname{cosec} \theta) = 2$$

$$(v) (\sin A + \operatorname{cosec} A)^2 + (\cos A + \sec A)^2 = 7 + \tan^2 A + \cot^2 A$$

$$(vi) \frac{\tan \theta + \sin \theta}{\tan \theta - \sin \theta} = \frac{\sec \theta + 1}{\sec \theta - 1} \quad (vii) \frac{\cot A - \cos A}{\cot A + \cos A} = \frac{\operatorname{cosec} A - 1}{\operatorname{cosec} A + 1} \quad (viii) \sec A (1 - \sin A)(\sec A + \tan A) = 1$$

$$(ix) (\operatorname{cosec} \theta - \cot \theta)^2 = \frac{1 - \cos \theta}{1 + \cos \theta} \quad (x) \frac{1 + \sec A}{\sec A} = \frac{\sin^2 A}{1 - \cos A}$$

$$(xi) \frac{\cos A}{1 + \sin A} + \frac{1 + \sin A}{\cos A} = 2 \sec A \quad (xii) \frac{\sin \theta}{1 + \cos \theta} + \frac{1 + \cos \theta}{\sin \theta} = 2 \operatorname{cosec} \theta$$

$$(xiii) (\operatorname{cosec} A - \sin A)(\sec A - \cos A) = \frac{1}{\tan A + \cot A}$$

$$(xiv) \frac{\sin \theta}{1 - \cos \theta} = \operatorname{cosec} \theta + \cot \theta \quad (xv) \sqrt{\frac{1 - \sin \theta}{1 + \sin \theta}} = \sec \theta - \tan \theta \quad (xvi) \sqrt{\frac{1 + \cos \theta}{1 - \cos \theta}} = \operatorname{cosec} \theta + \cot \theta$$

$$(xvii) \sqrt{\frac{1 + \sin \theta}{1 - \sin \theta}} = \sec \theta + \tan \theta \quad (xviii) \frac{\sin \theta - 2 \sin^3 \theta}{2 \cos^3 \theta - \cos \theta} = \tan \theta \quad (xix) \sec^2 \theta - \frac{\sin^2 \theta - 2 \sin^4 \theta}{2 \cos^4 \theta - \cos^2 \theta} = 1$$

$$(xx) \frac{\tan \theta}{1 - \cot \theta} + \frac{\cot \theta}{1 - \tan \theta} = 1 + \tan \theta + \cot \theta = 1 + \sec \theta \operatorname{cosec} \theta$$

$$(xxi) \frac{\cos A - \sin A + 1}{\cos A + \sin A - 1} = \operatorname{cosec} A + \cot A \quad (xxii) \frac{\sin \theta - \cos \theta + 1}{\sin \theta + \cos \theta - 1} = \frac{1}{\sec \theta - \tan \theta}$$

$$(xxiii) \left(\frac{1 + \tan^2 A}{1 + \cot^2 A} \right) = \left(\frac{1 - \tan A}{1 - \cot A} \right)^2 = \tan^2 A$$